\section{Lecture 20 (May 19th)}
\begin{thm}
Let there be an energy state $\hat{H}|E\rangle =E|E\rangle $. We previously found how
\[\hat{H}(\hat{a}|E\rangle )=(E-\hbar \omega )(\hat{a}|E\rangle )\]
and
\[\hat{H}(a^{\dagger}|E\rangle )=(E+\hbar \omega )(\hat{a}^{\dagger}|E\rangle )\]
Which needs to be verified. We have previously proved
\[\langle \psi |\hat{H}|\psi \rangle \geq 0\]
and tells us that there is a limit to how much the energy can be lowered. We thus define
\[\hat{a}|0\rangle ={\bf 0}\]
as the ground state, where ${\bf 0}$ is the zero vector. A simple corollary would be that
\[\hat{H}|0\rangle =(\hbar \omega )(\hat{a}^{\dagger}\hat{a})|0\rangle =\dfrac{1}{2}\hbar \omega |0\rangle \]
telling us that the ground state has an energy of $\hbar \omega /2$. We can apply the creation operator to obtain higher energy states:
\[H(\hat{a}^{\dagger}|0\rangle )=\Big(\dfrac{1}{2}\hbar \omega +\hbar \omega \Big)(\hat{a}^{\dagger}|0\rangle )\]
For arbitrary states,
\[E_{n}=\hbar \omega \Big(n+\dfrac{1}{2}\Big)\]
and
\[|n\rangle =c_{n}(\hat{a}^{\dagger})^{n}|0\rangle \]
We now prove that these eigenvectors form an orthonormal basis. The inner product of two eigenstates are
\[\langle m|n\rangle =c_{m}^{*}c_{n}\langle 0|a^{m}(a^{\dagger})^{n}|0\rangle =c_{m}^*c_{n}n\langle 0|a^{m-1}(a^{\dagger})^{n-1}|0\rangle \]
as $a^{m-1}a(a^{\dagger})^{n}=((a^{\dagger})^{n})a+[a,(a^{\dagger})^{n}])=((a^{\dagger})^{n}a+n(a^{\dagger})^{n-1})$. Therefore, when $n\ne m$, we find $\langle n|m\rangle =0$ and if they are equal,
\[\langle n|m\rangle =|c_{n}|^2n\langle 0|a^{n-1}(a^{\dagger})^{n-1}|0\rangle =|c_{n}|^2n(n-1)\langle 0|a^{n-1}(a^{\dagger})^{n-2}|0\rangle =\ldots =|c_{n}|^2n!\langle 0|0\rangle =1\]
thus getting something we should definitely memorise,
\[|n\rangle =\dfrac{1}{\sqrt{n!}}(a^{\dagger})^{n}|0\rangle \]
with $\langle n|m\rangle =\delta_{nm}$. Let's not find the annihilator operators matrix representation.
\begin{align*}
\langle m|a|n\rangle =&\langle m|a\cdot \dfrac{(a^{\dagger})^{n}}{\sqrt{n!}}|0\rangle =\dfrac{1}{\sqrt{n!}}\langle m|(a^{\dagger})^{n}a+a(a^{\dagger})^{n}|0\rangle \\
=&\dfrac{n}{\sqrt{n!}}\langle m|(a^{\dagger})^{n-1}|0\rangle=\dfrac{n}{\sqrt{n!}}\sqrt{(n-1)!}\langle m|\dfrac{(a^{\dagger})^{n-1}}{\sqrt{(n-1)!}}|0\rangle\\ =&\sqrt{n}\,\delta _{m,n-1}
\end{align*}
We can use the above to also obtain the creator operator's matrix representation, where
\[\langle m|\hat{a}^{\dagger}|n\rangle =\langle \hat{a}m|n\rangle =\langle n|a|m\rangle ^{*}=(\delta _{n,m-1}\sqrt{m})^{*}=\delta _{n,m-1}\sqrt{m}=\delta _{m+1,n}\sqrt{n+1}\]
\end{thm}
\vspace{2ex}
\begin{thm}
What is the wavefunction of the ground state? Mathematically, what is $\psi _{0}=\langle x|0\rangle $? 
\[\hat{a}|0\rangle =0\rightarrow \Big(\sqrt{\dfrac{m\omega }{2\hbar }}\hat{x}+i\sqrt{\dfrac{1}{2m\omega \hbar }}\hat{p}\Big)|0\rangle=0 \]
which leads to
\[\Big[\sqrt{\dfrac{m\omega }{2\hbar }}x+i\sqrt{\dfrac{1}{2m\omega \hbar }}\Big(-i\hbar \dfrac{d }{d x} \Big)\Big]\langle x|0\rangle =0\]
and
\[\langle x|0\rangle =c\exp \Big(-\dfrac{m\omega x^2}{2\hbar }\Big)\]
which must be normalised with
\[\int ^{\infty }_{-\infty }|\langle x|0\rangle |^2=1\quad \mathrm{and}\quad c=\Big(\dfrac{m\omega }{\pi \hbar }\Big)^{1/4}\]
To find higher wave functions,
\[\psi _{n}(x)=\langle x|n\rangle\]
try and compute this with $n=1$. 
\end{thm}
\vspace{2ex}
\begin{defi}
Define the exponential of an operator as
\[\exp (\hat{A})=\sum ^{\infty }_{n=0}\dfrac{1}{n!}(\hat{A})^{n}\]
Define the operator $\hat{U}=\exp (i\hat{A})$ for a Hermitian $\hat{A}$. We find that
\[\hat{U}^{\dagger}=(\sum ^{\infty }_{n=0}(-i)^{n}\hat{A}^{n})=\exp (-i\hat{A})=\hat{U}^{-1}\]
Therefore,
\[\hat{U}^{\dagger}\hat{U}={\bf 1}\]
and $\hat{U}$ is a unitary operator. 
\end{defi}
\vspace{2ex}
\begin{thm}
(Commuting set of operators and degeneracy) Here, we consider Hilbert spaces that are completely spanned by eigenstates of Hermitian operators. Take 
\[\hat{A}|u_{a}\rangle =a|u_{a}\rangle \]
which also satisfies
\[\hat{B}|u_{a}\rangle =b|u_{a}\rangle \]
Completeness dictates that
\[\sum _{a,b}|u_{ab}\rangle \langle u_{ab}|={\bf 1}\]
then, 
\[[\hat{A},\hat{B}]|u_{ab}\rangle =(\hat{A}\hat{B}-\hat{B}\hat{A})|u_{ab}\rangle =(ab-ba)|u_{ab}\rangle =0\]
telling us that $[\hat{A},\hat{B}]=0$.
\end{thm}
\vspace{2ex}

